refactor

execution/tests/ChainGens.v
@@ -6,6 +6,9 @@ From ConCert Require Import Blockchain.
 From ConCert Require Import LocalBlockchain.
 From ConCert Require Import Serializable.
 From ConCert Require Import BoundedN ChainedList.
+
+From ConCert.Execution.QCTests Require Import TestUtils ChainPrinting.
+
 (* For monad notations *)
 Require Export ExtLib.Structures.Monads.
 Export MonadNotation. Open Scope monad_scope.
@@ -19,82 +22,11 @@ Import LocalBlockchain.
 Import ListNotations.
 Close Scope address_scope.
 
-Definition AddrSize := (2^8)%N.
-Print ContractAddrBase.
-(* Let ContractAddrBase : N := @ContractAddrBase AddrSize. *)
 Instance LocalChainBase : ChainBase := LocalChainBase AddrSize.
 Instance LocalChainBuilder : ChainBuilderType := LocalChainBuilderDepthFirst AddrSize.
 
 
-Record ChainContext (BaseTypes : ChainBase) := 
-  mkBaseGens {
-    gAddress              : G (@Address BaseTypes);
-    accounts              : list (@Address BaseTypes);
-    contracts             : list (@Address BaseTypes);
-    gContractAddr         : G (@Address BaseTypes);
-    gAccountAddr          : G (@Address BaseTypes);    
-  }.
-  
-(* Helpers for ChainContext *)
-Definition ctx_gAccountAddr (ctx : ChainContext LocalChainBase) : G (@Address LocalChainBase) := 
-  @gAccountAddr LocalChainBase ctx.
-Definition ctx_gContractAddr (ctx : ChainContext LocalChainBase) : G (@Address LocalChainBase) := 
-  @gContractAddr LocalChainBase ctx.
-Definition ctx_gAnyAddr (ctx : ChainContext LocalChainBase) : G (@Address LocalChainBase) := 
-  @gAddress LocalChainBase ctx.
-Definition ctx_accounts (ctx : ChainContext LocalChainBase) : list Address := 
-  @accounts LocalChainBase ctx.
-Definition ctx_contracts (ctx : ChainContext LocalChainBase) : list Address := 
-  @contracts LocalChainBase ctx.
-
-Open Scope string_scope.
-
-Instance showBaseGens {BaseTypes : ChainBase} : Show (ChainContext BaseTypes)  :=
-  {|
-    show bg := "ChainContext{...}"
-  |}.
-
-Instance shrinkAmount : Shrink Amount := 
-  {|
-    shrink := @shrink Z _
-  |}.
-
-Definition empty_str : string := "".
-Definition sep : string := ", ".
-
-Instance showChain (BaseTypes : ChainBase) : Show (@Chain BaseTypes) :=
-  {|
-    show c := 
-      let height := show (chain_height c) in
-      let slot := show (current_slot c) in
-      let fin_height := show (finalized_height c) in
-        "Chain{" ++ "height: "       ++ height     ++ sep 
-                 ++ "current slot: " ++ slot       ++ sep 
-                 ++ "final height: " ++ fin_height ++ "}"
-  |}.
-
-Instance showEnvironment (BaseTypes : ChainBase) `{Show Chain}: Show Environment :=
-  {|
-    show env := "Environment{" 
-                ++ "chain: " ++ show (env_chain env) ++ sep 
-                ++ "contract states:..."             ++ "}"
-  |}.
-
-Close Scope string_scope.
 Open Scope list_scope.
-
-Fixpoint mkMapFromLists {A B : Type}
-                       (a_eqb : A -> A -> bool)
-                       (default : B)
-                       (l : list A) 
-                       (lb : list B)
-                       : A -> B :=
-  match (l,lb) with
-  | ([],[]) => fun x => default
-  | (a::l', b::lb') => 
-    fun (x : A) => if a_eqb x a then b else (mkMapFromLists a_eqb default l' lb') x 
-  | (_,_) => fun x => default
-  end.
 
 (* returns a generator in the given interval (inclusive).
    If low > high, then it will always generate the value high *)
@@ -125,43 +57,6 @@ Definition mkChainStateGen (BaseTypes : ChainBase)
                            : G ChainState 
   := returnGen (@build_chain_state BaseTypes env actionList).
 
-
-Derive Arbitrary for SerializedType.
-Derive Show for SerializedType.
-Import SerializedType.
-Open Scope string_scope.
-
-Fixpoint string_of_interp_type (st : SerializedType) :  (interp_type st) -> string :=
-match st as st0 return interp_type st0 -> string with
-  | ser_unit => fun _ => "()"
-  | ser_int => fun t => show t
-  | ser_bool => fun t => show t
-  | ser_list a => 
-    fun t : list (interp_type a) => 
-      let t_str_list := map (string_of_interp_type a) t in 
-      "[" ++ String.concat ";" t_str_list ++ "]"  
-  | ser_pair a b => 
-    fun t : (interp_type a * interp_type b) => 
-      "(" 
-      ++ string_of_interp_type a (fst t) 
-      ++ ","
-      ++ string_of_interp_type b (snd t) ++ ")"
-  end.  
-
-Definition ex_serialized_type := ser_pair (ser_list (ser_list ser_bool)) ser_int.
-Compute (interp_type ex_serialized_type).
-Definition ex_val := ([[true;false];[true;true];[false];[]], 2%Z).
-Compute (string_of_interp_type ex_serialized_type ex_val).
-
-Close Scope list_scope.
-Instance showSerializedValue : Show SerializedValue := 
-  {|
-    show v := "SerializedValue{" 
-              (* ++ show (ser_value_type v) ++ sep *)
-              ++ string_of_interp_type (ser_value_type v) (ser_value v) ++ "}" 
-  |}.
-Close Scope string_scope.
-
 Fixpoint gInterp_type (t : SerializedType) : G (interp_type t) := 
   match t with
   | ser_unit => returnGen tt
@@ -170,6 +65,8 @@ Fixpoint gInterp_type (t : SerializedType) : G (interp_type t) :=
   | ser_pair a b => liftM2 pair (gInterp_type a) (gInterp_type b) 
   | ser_list a => listOf (gInterp_type a)
   end.
+
+Derive Arbitrary for SerializedType.
 
 Definition gSerializedValueSized (n : nat): G SerializedValue :=
   t <- arbitrarySized n ;;
@@ -293,48 +190,7 @@ Definition gActionFromContract  {Setup Msg State : Type}
 Definition zero_address : Address := BoundedN.of_Z_const AddrSize 0.
 Definition b9 : option (BoundedN.BoundedN AddrSize) := @BoundedN.of_nat AddrSize 9.
 
-(* Show instances *)
-Open Scope string_scope.
-
-(* We dont show the bound because it may be a very large number which, when converted to nat and then to string, gives a memory overflow. *)
-Instance showBoundedN {bound : N} `{Show N} : Show (BoundedN.BoundedN bound) :=
-  {|
-    show bn := match bn with | BoundedN.bounded n _ => show n ++ "%" ++ show bound end  
-  |}.
- 
-
-Instance showBoundedNAddrSize : Show (BoundedN.BoundedN AddrSize) :=
-  {|
-    show := @show (BoundedN.BoundedN AddrSize) showBoundedN
-  |}.
-
-Instance showAddress : Show (@Address LocalChainBase) :=
-  {|
-    show := @show (BoundedN.BoundedN AddrSize) showBoundedNAddrSize
-  |}.
-
-Compute (show zero_address).
-
-Instance showLocalChain : Show (@LocalChain AddrSize) := 
-  {|
-    show lc := "LocalChain{" 
-                ++ show (lc_height lc) ++ sep 
-                ++ show (lc_slot lc)   ++ sep 
-                ++ show (lc_fin_height lc) 
-                ++ sep ++ "... }"
-  |}.
-
-Instance showLocalContractCallContext : Show (@ContractCallContext LocalChainBase) :=
-{|
-  show cctx := "ContractCallContext{"
-               ++ "ctx_from: " ++ show (@ctx_from LocalChainBase cctx) ++ sep
-               ++ "ctx_contract_addr: " ++ show (@ctx_contract_address LocalChainBase cctx) ++ sep
-               ++ "ctx_amount: " ++ show (@ctx_amount LocalChainBase cctx) ++ "}"
-|}.
-
-Close Scope string_scope.
-
-Derive Show for positive.
+Derive Arbitrary for SerializedType.
 Derive Arbitrary for positive.
 Derive GenSized for positive.
 
@@ -435,26 +291,10 @@ Open Scope list_scope.
 Definition acc_bal := mkMapFromLists (fun x y => x =? y) 42 [10;20;30;40] [1;2;3;4].
 Definition testGChain : G Chain := ctx <- arbitrary ;; gLocalChainSized 2 ctx.
 
-Sample (gLocalChainContext 10).
-
 (* Sample (@arbitrarySized Chain _ 2). *)
-Sample (bh <- gLocalChainContext 2 ;; @gAddress LocalChainBase bh). (* IMPORTANT NOTE: if we omit the explicit types, it will not work *)
+Sample (bh <- gLocalChainContext 1 ;; @gAddress LocalChainBase bh). (* IMPORTANT NOTE: if we omit the explicit types, it will not work *)
 Sample (gEnvFromLocalChain lc_initial).
 
-Open Scope string_scope.
-(* Show and Generator instances for types related to Traces (an execution sequence of contracts on the BC) *)
-Instance showBlockHeader (BaseTypes : ChainBase) `{Show (@Address BaseTypes)} : Show (@BlockHeader BaseTypes) :=
-  {|
-    show bh := 
-      "BlockHeader{" ++ "bheight: "     ++ show (block_height bh)           ++ sep
-                     ++ "bslot: "       ++ show (block_slot bh)             ++ sep 
-                     ++ "bfin_height: " ++ show (block_finalized_height bh) ++ sep
-                     ++ "breward: "     ++ show (block_reward bh)           ++ sep
-                     ++ "bcreator: "    ++ show (block_creator bh)          ++ "}" 
-  |}.
-
-
-Close Scope string_scope.
 
 (* make a generator for a BlockHeader from a given chain.
    Should satisfy the IsValidNextBlock predicate. *)
@@ -485,11 +325,10 @@ Definition gLocalBCBlockHeaderSizedFromChainAndContext : nat ->
 Definition blockHeader_ex : (@BlockHeader LocalChainBase) := build_block_Header 0 0 0 0 zero_address.
 Definition gbh_dummy := returnGen blockHeader_ex.
 
-Compute (show blockHeader_ex).
 Sample gbh_dummy.
-Sample (ctx <- arbitrary ;; @gContractCallContext LocalChainBase ctx).
+(* Sample (ctx <- arbitrary ;; @gContractCallContext LocalChainBase ctx). *)
 
-Sample (ctx <- arbitrary ;; c <- gLocalChainSized 2 ctx ;; gLocalBCBlockHeaderSizedFromChainAndContext 2 c ctx).
+Sample (ctx <- arbitrary ;; c <- gLocalChainSized 1 ctx ;; gLocalBCBlockHeaderSizedFromChainAndContext 1 c ctx).
 
 Definition validate_header_P : BlockHeader * Chain -> bool :=  fun p => match validate_header (fst p) (snd p) with Some _ => true | None => false end.
 
