execution/tests/ChainPrinting.v
@@ -1,0 +1,141 @@
+Require Import ZArith Strings.Ascii Strings.String.
+From QuickChick Require Import QuickChick. Import QcNotation.
+From ExtLib.Structures Require Import Functor Applicative.
+
+From ConCert Require Import Blockchain.
+From ConCert Require Import LocalBlockchain.
+From ConCert Require Import Serializable. Import SerializedType.
+From ConCert Require Import BoundedN ChainedList.
+
+From ConCert.Execution.QCTests Require Import TestUtils.
+
+(* For monad notations *)
+Require Export ExtLib.Structures.Monads.
+Export MonadNotation. Open Scope monad_scope.
+
+From Coq Require Import List.
+From Coq Require Import Strings.BinaryString.
+From Coq Require Import Morphisms.
+Import BoundedN.Stdpp.
+
+Import LocalBlockchain.
+Import ListNotations.
+Close Scope address_scope.
+
+Definition AddrSize := (2^8)%N.
+Instance LocalChainBase : ChainBase := LocalChainBase AddrSize.
+Instance LocalChainBuilder : ChainBuilderType := LocalChainBuilderDepthFirst AddrSize.
+
+Open Scope list_scope.
+Open Scope string_scope.
+
+Derive Show for positive.
+Derive Show for SerializedType.
+
+Instance showBaseGens {BaseTypes : ChainBase} : Show (ChainContext BaseTypes)  :=
+  {|
+    show bg := "ChainContext{...}"
+  |}.
+
+Instance shrinkAmount : Shrink Amount := 
+  {|
+    shrink := @shrink Z _
+  |}.
+
+  Instance showChain (BaseTypes : ChainBase) : Show (@Chain BaseTypes) :=
+  {|
+    show c := 
+      let height := show (chain_height c) in
+      let slot := show (current_slot c) in
+      let fin_height := show (finalized_height c) in
+        "Chain{" ++ "height: "       ++ height     ++ sep 
+                 ++ "current slot: " ++ slot       ++ sep 
+                 ++ "final height: " ++ fin_height ++ "}"
+  |}.
+
+Instance showEnvironment (BaseTypes : ChainBase) `{Show Chain}: Show Environment :=
+  {|
+    show env := "Environment{" 
+                ++ "chain: " ++ show (env_chain env) ++ sep 
+                ++ "contract states:..."             ++ "}"
+  |}.
+
+
+Fixpoint string_of_interp_type (st : SerializedType) :  (interp_type st) -> string :=
+match st as st0 return interp_type st0 -> string with
+  | ser_unit => fun _ => "()"
+  | ser_int => fun t => show t
+  | ser_bool => fun t => show t
+  | ser_list a => 
+    fun t : list (interp_type a) => 
+      let t_str_list := map (string_of_interp_type a) t in 
+      "[" ++ String.concat ";" t_str_list ++ "]"  
+  | ser_pair a b => 
+    fun t : (interp_type a * interp_type b) => 
+      "(" 
+      ++ string_of_interp_type a (fst t) 
+      ++ ","
+      ++ string_of_interp_type b (snd t) ++ ")"
+  end.  
+
+Definition ex_serialized_type := ser_pair (ser_list (ser_list ser_bool)) ser_int.
+(* Compute (interp_type ex_serialized_type). *)
+Definition ex_val := ([[true;false];[true;true];[false];[]], 2%Z).
+(* Compute (string_of_interp_type ex_serialized_type ex_val). *)
+
+Instance showSerializedValue : Show SerializedValue := 
+{|
+  show v := "SerializedValue{" 
+  (* ++ show (ser_value_type v) ++ sep *)
+  ++ string_of_interp_type (ser_value_type v) (ser_value v) ++ "}" 
+|}.
+
+(* Show and Generator instances for types related to Traces (an execution sequence of contracts on the BC) *)
+Instance showBlockHeader (BaseTypes : ChainBase) `{Show (@Address BaseTypes)} : Show (@BlockHeader BaseTypes) :=
+  {|
+    show bh := 
+      "BlockHeader{" ++ "bheight: "     ++ show (block_height bh)           ++ sep
+                     ++ "bslot: "       ++ show (block_slot bh)             ++ sep 
+                     ++ "bfin_height: " ++ show (block_finalized_height bh) ++ sep
+                     ++ "breward: "     ++ show (block_reward bh)           ++ sep
+                     ++ "bcreator: "    ++ show (block_creator bh)          ++ "}" 
+  |}.
+
+  (* We dont show the bound because it may be a very large number which, when converted to nat and then to string, gives a memory overflow. *)
+Instance showBoundedN {bound : N} `{Show N} : Show (BoundedN.BoundedN bound) :=
+{|
+  show bn := match bn with | BoundedN.bounded n _ => show n ++ "%" ++ show bound end  
+|}.
+
+
+Instance showBoundedNAddrSize : Show (BoundedN.BoundedN AddrSize) :=
+{|
+  show := @show (BoundedN.BoundedN AddrSize) showBoundedN
+|}.
+
+Instance showAddress : Show (@Address LocalChainBase) :=
+{|
+  show := @show (BoundedN.BoundedN AddrSize) showBoundedNAddrSize
+|}.
+
+
+Instance showLocalChain : Show (@LocalChain AddrSize) := 
+{|
+  show lc := "LocalChain{" 
+              ++ show (lc_height lc) ++ sep 
+              ++ show (lc_slot lc)   ++ sep 
+              ++ show (lc_fin_height lc) 
+              ++ sep ++ "... }"
+|}.
+
+Instance showLocalContractCallContext : Show (@ContractCallContext LocalChainBase) :=
+{|
+show cctx := "ContractCallContext{"
+             ++ "ctx_from: " ++ show (@ctx_from LocalChainBase cctx) ++ sep
+             ++ "ctx_contract_addr: " ++ show (@ctx_contract_address LocalChainBase cctx) ++ sep
+             ++ "ctx_amount: " ++ show (@ctx_amount LocalChainBase cctx) ++ "}"
+|}.
+
+
+Close Scope string_scope.
+Close Scope list_scope.
