execution/tests/TestUtils.v
@@ -1,0 +1,160 @@
+Require Import ZArith Strings.Ascii Strings.String.
+From QuickChick Require Import QuickChick. Import QcNotation.
+From ExtLib.Structures Require Import Functor Applicative.
+Require Export ExtLib.Structures.Monads.
+Export MonadNotation. Open Scope monad_scope.
+
+From ConCert Require Import Blockchain.
+From ConCert Require Import LocalBlockchain.
+From ConCert Require Import Serializable. Import SerializedType.
+From ConCert Require Import BoundedN ChainedList.
+
+
+
+From Coq Require Import List. Import ListNotations.
+From Coq Require Import Program.Basics.
+Require Import Containers.
+
+Global Definition AddrSize := (2^8)%N.
+Instance LocalChainBase : ChainBase := LocalChainBase AddrSize.
+Instance LocalChainBuilder : ChainBuilderType := LocalChainBuilderDepthFirst AddrSize.
+
+Notation "f 'o' g" := (compose f g) (at level 50).
+
+
+(* Misc utility functions *)
+Open Scope list_scope.
+Open Scope string_scope.
+
+Fixpoint mkMapFromLists {A B : Type}
+                       (a_eqb : A -> A -> bool)
+                       (default : B)
+                       (l : list A) 
+                       (lb : list B)
+                       : A -> B :=
+  match (l,lb) with
+  | ([],[]) => fun x => default
+  | (a::l', b::lb') => 
+    fun (x : A) => if a_eqb x a then b else (mkMapFromLists a_eqb default l' lb') x 
+  | (_,_) => fun x => default
+  end.
+
+Definition string_of_FMap {A B : Type}
+                         `{countable.Countable A}
+                         `{base.EqDecision A}
+                          (showA : A -> string) 
+                          (showB : B -> string) 
+                          (m : FMap A B) : string :=
+  show (map (fun p => showA (fst p) ++ "-->" ++ showB (snd p)) (FMap.elements m)).
+
+
+(* Utils for Show instances *)
+
+Definition empty_str : string := "".
+Definition sep : string := ", ".
+Derive Show for unit.
+
+Definition deserialize_to_string (s : SerializedValue) : string := 
+  match deserialize s with
+  | Some v => show v
+  | None => "?"
+  end.
+
+Instance showFMap {A B : Type}
+                 `{countable.Countable A}
+                 `{base.EqDecision A}
+                 `{Show A} 
+                 `{Show B}
+                  : Show (FMap A B) :=
+{|
+  show := string_of_FMap show show
+|}.
+
+Close Scope string_scope.
+
+
+(* Utils for Generators *)
+
+
+Record ChainContext (BaseTypes : ChainBase) := 
+  mkBaseGens {
+    gAddress              : G (@Address BaseTypes);
+    accounts              : list (@Address BaseTypes);
+    contracts             : list (@Address BaseTypes);
+    gContractAddr         : G (@Address BaseTypes);
+    gAccountAddr          : G (@Address BaseTypes);    
+  }.
+  
+(* Helpers for ChainContext. TODO: look into parameterising ChainBase *)
+Definition ctx_gAccountAddr (ctx : ChainContext LocalChainBase) : G (@Address LocalChainBase) := 
+  @gAccountAddr LocalChainBase ctx.
+Definition ctx_gContractAddr (ctx : ChainContext LocalChainBase) : G (@Address LocalChainBase) := 
+  @gContractAddr LocalChainBase ctx.
+Definition ctx_gAnyAddr (ctx : ChainContext LocalChainBase) : G (@Address LocalChainBase) := 
+  @gAddress LocalChainBase ctx.
+Definition ctx_accounts (ctx : ChainContext LocalChainBase) : list Address := 
+  @accounts LocalChainBase ctx.
+Definition ctx_contracts (ctx : ChainContext LocalChainBase) : list Address := 
+  @contracts LocalChainBase ctx.
+
+Definition gZPositive := liftM Z.of_nat arbitrary.
+Definition gZPositiveSized n := liftM Z.of_nat (arbitrarySized n).
+
+(* Helper generator and show instance for arbitrary FMaps *)
+
+Fixpoint gFMapSized {A B : Type} 
+                    {gA : G A} 
+                    {gB : G B}
+                    `{countable.Countable A}
+                    `{base.EqDecision A}
+                     (n : nat) : G (FMap A B) :=
+  match n with
+  | 0 => returnGen FMap.empty
+  | S n' =>
+    a <- gA ;;
+    b <- gB ;;
+    m <- @gFMapSized _ _ gA gB _ _ _ n' ;;
+    returnGen (FMap.add a b m)  
+  end.
+
+Fixpoint gFMapFromInput {A B : Type}
+                       `{countable.Countable A}
+                       `{base.EqDecision A}     
+                        (l1 : list A)
+                        (l2 : list B)
+                        : G (FMap A B) :=
+  match (l1, l2) with
+  | (a::l1', b::l2') => liftM (FMap.add a b) (gFMapFromInput l1' l2')
+  | (_, _) => returnGen FMap.empty
+  end.
+
+Instance genFMapSized {A B : Type} 
+                     `{Gen A} 
+                     `{Gen B}
+                     `{countable.Countable A}
+                     `{base.EqDecision A}
+                      : GenSized (FMap A B) :=
+{|
+  arbitrarySized := @gFMapSized A B arbitrary arbitrary _ _ _
+|}.
+
+Sample (@gFMapSized nat nat arbitrary arbitrary _ _ _ 1).
+
+
+Fixpoint vectorOfCount {A : Type}
+                      `{countable.Countable A} 
+                       (default : A)
+                       (n : nat) : G (list A) := 
+  match n with
+  | 0    => returnGen []
+  | S n' => 
+    match (countable.decode o Pos.of_nat) n with
+    | Some a => liftM (cons a) (vectorOfCount default n')
+    | None => liftM (cons default) (vectorOfCount default n')
+    end
+  end.
+
+
+(* Utils for QuickChick *)
+
+Close Scope list_scope.
